feat(F* extraction): functional correctness

libcrux-ml-dsa/proofs/fstar/extraction/Libcrux_ml_dsa.Simd.Portable.Encoding.Commitment.fsti
@@ -3,7 +3,90 @@ module Libcrux_ml_dsa.Simd.Portable.Encoding.Commitment
 open Core
 open FStar.Mul
 
+val encode_4_ (coefficients: t_Slice i32)
+    : Prims.Pure u8
+      (requires Seq.length coefficients == 2 /\ (forall i. bounded (Seq.index coefficients i) 4))
+      (ensures
+        fun out ->
+          let out:u8 = out in
+          let inp = bit_vec_of_int_t_array #I32 #(mk_usize 2) coefficients 4 in
+          let out = bit_vec_of_int_t_array #U8 (MkSeq.create1 out) 8 in
+          forall (i: nat{i < 8}). inp i == out i)
+
+val encode_6_ (coefficients: t_Slice i32)
+    : Prims.Pure (u8 & u8 & u8)
+      (requires Seq.length coefficients == 4 /\ (forall i. bounded (Seq.index coefficients i) 6))
+      (ensures
+        fun out ->
+          let out:(u8 & u8 & u8) = out in
+          let inp = bit_vec_of_int_t_array #I32 #(mk_usize 4) coefficients 6 in
+          let out = bit_vec_of_int_t_array #U8 (MkSeq.create3 out) 8 in
+          forall (i: nat{i < 8 * 3}). inp i == out i)
+
+val serialize_4_
+      (simd_unit: Libcrux_ml_dsa.Simd.Portable.Vector_type.t_Coefficients)
+      (serialized: t_Slice u8)
+    : Prims.Pure (t_Slice u8)
+      (requires
+        Seq.length serialized == 4 /\
+        (forall i.
+            bounded (Seq.index simd_unit.Libcrux_ml_dsa.Simd.Portable.Vector_type.f_values i) 4))
+      (ensures
+        fun serialized_future ->
+          let serialized_future:t_Slice u8 = serialized_future in
+          let serialized_future:t_Slice u8 = serialized_future in
+          Seq.length serialized_future == Seq.length serialized /\
+          (let inp =
+              bit_vec_of_int_t_array #I32
+                #(mk_usize 8)
+                simd_unit.Libcrux_ml_dsa.Simd.Portable.Vector_type.f_values
+                4
+            in
+            let out = bit_vec_of_int_t_array #U8 #(mk_usize 4) serialized_future 8 in
+            forall (i: nat{i < 8 * 4}). inp i == out i))
+
+val serialize_6_
+      (simd_unit: Libcrux_ml_dsa.Simd.Portable.Vector_type.t_Coefficients)
+      (serialized: t_Slice u8)
+    : Prims.Pure (t_Slice u8)
+      (requires
+        Seq.length serialized == 6 /\
+        (forall i.
+            bounded (Seq.index simd_unit.Libcrux_ml_dsa.Simd.Portable.Vector_type.f_values i) 6))
+      (ensures
+        fun serialized_future ->
+          let serialized_future:t_Slice u8 = serialized_future in
+          let serialized_future:t_Slice u8 = serialized_future in
+          Seq.length serialized_future == Seq.length serialized /\
+          (let inp =
+              bit_vec_of_int_t_array #I32
+                #(mk_usize 8)
+                simd_unit.Libcrux_ml_dsa.Simd.Portable.Vector_type.f_values
+                6
+            in
+            let out = bit_vec_of_int_t_array #U8 #(mk_usize 6) serialized_future 8 in
+            forall (i: nat{i < 8 * 6}). inp i == out i))
+
 val serialize
       (simd_unit: Libcrux_ml_dsa.Simd.Portable.Vector_type.t_Coefficients)
       (serialized: t_Slice u8)
-    : Prims.Pure (t_Slice u8) Prims.l_True (fun _ -> Prims.l_True)
+    : Prims.Pure (t_Slice u8)
+      (requires
+        (let d = Seq.length serialized in
+          (d == 4 \/ d == 6) /\
+          (forall i.
+              bounded (Seq.index simd_unit.Libcrux_ml_dsa.Simd.Portable.Vector_type.f_values i) d)))
+      (ensures
+        fun serialized_future ->
+          let serialized_future:t_Slice u8 = serialized_future in
+          let serialized_future:t_Slice u8 = serialized_future in
+          let d = Seq.length serialized in
+          (Seq.length serialized_future == d /\
+            (let inp =
+                bit_vec_of_int_t_array #I32
+                  #(mk_usize 8)
+                  simd_unit.Libcrux_ml_dsa.Simd.Portable.Vector_type.f_values
+                  d
+              in
+              let out = bit_vec_of_int_t_array #U8 #(mk_usize d) serialized_future 8 in
+              forall (i: nat{i < 8 * d}). inp i == out i)))
